started with int types and fallible encode.

defs.v
@@ -1,31 +1,48 @@
-Require Import Coq.Bool.Bool.
-Require Import Coq.Init.Datatypes.
+Require Import Bool.
+Require Import Datatypes.
 Require Import Coq.Init.Byte.
-Require Import Coq.Lists.List.
+Require Import ZArith.
+Require Import List.
 Import ListNotations.
 
 (* provenance *)
 Context `{P : Type}.
 
+(* in bytes *)
+Definition Size := nat.
+
+Definition Int := Z.
+
+Inductive Signedness :=
+ | Signed : Signedness
+ | Unsigned : Signedness.
+
 Inductive Ty : Type :=
- | BoolTy : Ty.
+ | BoolTy : Ty
+ | IntTy : Size -> Signedness -> Ty.
 
 Inductive Value : Type :=
- | BoolVal : bool -> Value.
+ | BoolVal : bool -> Value
+ | IntVal : Int -> Value.
 
 Inductive AbstractByte : Type :=
  | Uninit : AbstractByte
  | Init : byte -> option P -> AbstractByte.
 
-Definition encode (ty : Ty) (val: Value) : list AbstractByte :=
+(* TODO add ints! *)
+Definition encode (ty : Ty) (val: Value) : option (list AbstractByte) :=
  match (ty, val) with
-  | (BoolTy, BoolVal true) => [Init x01 None]
-  | (BoolTy, BoolVal false) => [Init x00 None]
+  | (BoolTy, BoolVal true) => Some [Init x01 None]
+  | (BoolTy, BoolVal false) => Some [Init x00 None]
+  | _ => None
  end.
 
+(* TODO add ints! *)
 Definition decode (ty : Ty) (bytes : list AbstractByte) : option Value :=
  match (ty, bytes) with
   | (BoolTy, [Init x01 _]) => Some (BoolVal true)
   | (BoolTy, [Init x00 _]) => Some (BoolVal false)
   | _ => None
  end.
+
+Definition is_valid_for (ty : Ty) (v : Value) := exists l, decode ty l = Some v.
