thm.v
@@ -8,17 +8,22 @@ Require Import Coq.Init.Byte.
 Require Import Coq.Lists.List.
 Import ListNotations.
 
-Theorem mono1 (ty: Ty) (v1 v2: Value) (p: le_val v1 v2) : le_list (encode ty v1) (encode ty v2).
+Theorem mono1 (ty: Ty) (v1 v2: Value) (p: le_val v1 v2) (p1: is_valid_for ty v1) (p2: is_valid_for ty v2) :
+exists e1, exists e2, encode ty v1 = Some e1 /\ encode ty v2 = Some e2 /\ le_list e1 e2.
 Proof.
+(*
 destruct v1,v2.
 unfold le_val in p.
 simpl in p.
 replace b0 with b.
 apply obvious.
 Qed.
+*)
+Abort.
 
 Theorem mono2 (ty: Ty) (l1 l2: list AbstractByte) (p: le_list l1 l2) : le_opt (decode ty l1) (decode ty l2).
 Proof.
+(*
 destruct ty.
 destruct (mk_le_list l1 l2 p) as [|x1 x2 l1' l2' p' H].
 - unfold le_opt,decode. assumption.
@@ -34,18 +39,24 @@ destruct (mk_le_list l1 l2 p) as [|x1 x2 l1' l2' p' H].
 -- unfold decode.
 destruct x1; destruct x2; try destruct b; unfold le_opt; auto.
 Qed.
+*)
+Abort.
 
-
-Theorem roundtrip1 (ty: Ty) (v: Value) : decode ty (encode ty v) = Some v.
+Theorem roundtrip1 (ty: Ty) (v: Value) (p: is_valid_for ty v) :
+exists e, encode ty v = Some e /\ decode ty e = Some v.
 Proof.
+(*
 destruct ty.
 destruct v.
 destruct b; unfold encode,decode; reflexivity.
 Qed.
+*)
+Abort.
 
-Theorem roundtrip2 (ty: Ty) (l: list AbstractByte) (v: Value) : (decode ty l = Some v) -> le_list (encode ty v) l. 
+Theorem roundtrip2 (ty: Ty) (l: list AbstractByte) (v: Value) (H: decode ty l = Some v) :
+exists e, encode ty v = Some e /\ le_list e l.
 Proof.
-intros H.
+(*
 destruct ty.
 destruct v.
 destruct (mk_decode_bool l).
@@ -57,3 +68,5 @@ destruct (mk_decode_bool l).
   unfold le_abstract_byte. reflexivity.
 - rewrite e in H. discriminate H.
 Qed.
+*)
+Abort.
